Bedrock/Platform/Facade/examples/Tuples1F.v
@@ -17,17 +17,147 @@ Definition keepGt (ts : tuples) (key k : W) : tuples :=
   fun tup => Ensembles.In _ ts tup /\ Array.sel (indexedElement tup) key > k.
 Definition empty (ts : tuples) := forall t, ~Ensembles.In _ ts t.
 
+Definition replaceKey (ts ts' : tuples) (key k : W) : tuples :=
+  fun t => IF Array.sel (indexedElement t) key = k then ts' t else ts t.
+
+Definition bounded (ts : tuples) := exists bound, UnConstrFreshIdx ts bound.
+
+Ltac Equiv' := unfold bounded, insert, EnsembleInsert, Equiv, replaceKey, IF_then_else,
+               keepEq, keepLt, keepGt, empty, Ensembles.In, UnConstrFreshIdx in *.
+Ltac Equiv := Equiv'; firstorder idtac.
+
+Theorem keepEq_Equiv : forall ts1 ts2 key k,
+  Equiv ts1 ts2
+  -> Equiv (keepEq ts1 key k) (keepEq ts2 key k).
+Proof.
+  Equiv.
+Qed.
+
+Theorem keepLt_Equiv : forall ts1 ts2 key k,
+  Equiv ts1 ts2
+  -> Equiv (keepLt ts1 key k) (keepLt ts2 key k).
+Proof.
+  Equiv.
+Qed.
+
+Theorem keepGt_Equiv : forall ts1 ts2 key k,
+  Equiv ts1 ts2
+  -> Equiv (keepGt ts1 key k) (keepGt ts2 key k).
+Proof.
+  Equiv.
+Qed.
+
+Hint Immediate keepEq_Equiv keepLt_Equiv keepGt_Equiv.
+
+Lemma Equiv_keepEq_replaceKey : forall k1 k ts key ts',
+  k1 < k
+  -> Equiv (keepEq ts key k) (keepEq (replaceKey ts ts' key k1) key k).
+Proof.
+  Equiv.
+  subst; right; intuition.
+  subst; nomega.
+  subst; nomega.
+Qed.
+
+Hint Immediate Equiv_keepEq_replaceKey.
+
+Lemma Equiv_keepGt_replaceKey_lt : forall k1 k ts key ts',
+  k1 < k
+  -> Equiv (keepGt ts' key k) (keepGt (replaceKey ts' ts key k1) key k).
+Proof.
+  Equiv.
+  right; intuition.
+  subst; nomega.
+  subst; nomega.
+Qed.
+
+Hint Immediate Equiv_keepGt_replaceKey_lt.
+
+(*Lemma Equiv_keepLt_replaceKey_lt : forall k1 k ts key ts' t,
+  k1 < k
+  -> insert (keepLt ts' key k) t ts
+  -> k1 = Array.sel t key
+  -> Equiv ts (keepLt (replaceKey ts' ts key k1) key k).
+Proof.
+  Equiv'.
+  intuition subst.
+
+  destruct H0; intuition subst.
+  specialize (proj1 (H3 _) H2).
+  intuition (subst; simpl in * ).
+  tauto.  
+  destruct (weq (Array.sel (indexedElement t0) key) (Array.sel t key)); tauto.
+
+  destruct H0; intuition subst.
+  specialize (proj1 (H3 _) H2).
+  intuition (subst; simpl in * ).
+  tauto.
+
+  destruct H0; intuition subst.
+  apply H2; tauto.
+Qed.
+
+Hint Immediate Equiv_keepLt_replaceKey_lt.
+
+Lemma bounded_insert : forall ts t ts',
+  insert ts t ts'
+  -> bounded ts
+  -> bounded ts'.
+Proof.
+  Equiv.
+  exists (S (max x x0)).
+  intros.
+  apply H1 in H2; intuition (subst; simpl).
+  specialize (Max.max_spec x x0); intuition.
+  apply H in H3.
+  specialize (Max.max_spec x x0); intuition.
+Qed.
+
+Hint Immediate bounded_insert.*)
+
+(*Lemma insert_replaceKey_lt : forall k1 k ts key ts' t,
+  k1 < k
+  -> insert (keepLt ts key k) t ts'
+  -> k1 = Array.sel t key
+  -> bounded ts
+  -> insert ts t (replaceKey ts ts' key k1).
+Proof.
+  Equiv'; intuition subst.
+  destruct H0, H2; intuition.
+  exists (max x x0); intuition (subst; simpl in * ).
+  apply H1 in H0; specialize (Max.max_spec x x0); intuition.
+  apply H3 in H5; intuition (subst; simpl in * ).
+
+  unfold EnsembleInsert in *; intuition subst.
+
+  unfold insert.
+  unfold EnsembleInsert.
+
+  intuition (subst; simpl in * ).
+  tauto.
+  destruct (weq (Array.sel (indexedElement t0) key) (Array.sel t key)); tauto.
+
+  intuition (subst; simpl in * ); auto.
+
+  tauto.
+Qed.*)
+
+
 Module Type ADT.
-  Parameter tuples1 : W -> tuples -> W -> HProp.
+  Parameter tuples1 : W -> W -> tuples -> W -> HProp.
   Parameter tree : W -> W -> skel -> tuples -> W -> HProp.
 
-  Axiom tuples1_fwd : forall len ts c, tuples1 len ts c
+  Axiom tuples1_fwd : forall len key ts c, tuples1 len key ts c
     ===> [| c <> 0 |] * [| freeable c 3 |] * [| $2 <= len |]
-        * Ex key, Ex p, Ex sk, (c ==*> len, key, p) * tree len key sk ts p * [| key < len |].
-  Axiom tuples1_bwd : forall len ts (c : W),
+        * Ex p, Ex sk, (c ==*> len, key, p) * tree len key sk ts p * [| key < len |].
+  Axiom tuples1_bwd : forall len key ts (c : W),
     ([| c <> 0 |] * [| freeable c 3 |] * [| $2 <= len |]
-    * Ex key, Ex p, Ex sk, (c ==*> len, key, p) * tree len key sk ts p * [| key < len |])
-    ===> tuples1 len ts c.
+    * Ex p, Ex sk, (c ==*> len, key, p) * tree len key sk ts p * [| key < len |])
+    ===> tuples1 len key ts c.
+
+  Axiom tree_Equiv : forall len key sk ts1 ts2 p,
+    Equiv ts1 ts2
+    -> tree len key sk ts1 p ===> tree len key sk ts2 p.
 
   Axiom tree_leaf_fwd : forall len key sk ts (p : W), p = 0
     -> tree len key sk ts p ===> [| sk = Leaf |] * [| empty ts |].
@@ -63,23 +193,35 @@ Module Adt : ADT.
         * tree len key sk2 (keepGt ts key k) p2
     end.
 
-  Definition tuples1 (len : W) (ts : tuples) (c : W) : HProp :=
+  Definition tuples1 (len key : W) (ts : tuples) (c : W) : HProp :=
     [| c <> 0 |] * [| freeable c 3 |] * [| $2 <= len |]
-    * Ex key, Ex p, Ex sk, (c ==*> len, key, p) * tree len key sk ts p * [| key < len |].
+    * Ex p, Ex sk, (c ==*> len, key, p) * tree len key sk ts p * [| key < len |].
 
-  Theorem tuples1_fwd : forall len ts c, tuples1 len ts c
+  Theorem tuples1_fwd : forall len key ts c, tuples1 len key ts c
     ===> [| c <> 0 |] * [| freeable c 3 |] * [| $2 <= len |]
-    * Ex key, Ex p, Ex sk, (c ==*> len, key, p) * tree len key sk ts p * [| key < len |].
+    * Ex p, Ex sk, (c ==*> len, key, p) * tree len key sk ts p * [| key < len |].
   Proof.
-    unfold tuples1; sepLemma.
+    unfold tuples1; sepLemma; eauto.
   Qed.
 
-  Theorem tuples1_bwd : forall len ts (c : W),
+  Theorem tuples1_bwd : forall len key ts (c : W),
     ([| c <> 0 |] * [| freeable c 3 |] * [| $2 <= len |]
-     * Ex key, Ex p, Ex sk, (c ==*> len, key, p) * tree len key sk ts p * [| key < len |])
-    ===> tuples1 len ts c.
+     * Ex p, Ex sk, (c ==*> len, key, p) * tree len key sk ts p * [| key < len |])
+    ===> tuples1 len key ts c.
   Proof.
-    unfold tuples1; sepLemma.
+    unfold tuples1; sepLemma; eauto.
+  Qed.
+
+  Theorem tree_Equiv : forall len key sk ts1 ts2 p,
+    Equiv ts1 ts2
+    -> tree len key sk ts1 p ===> tree len key sk ts2 p.
+  Proof.
+    induction sk; sepLemma.
+
+    Equiv.
+
+    repeat apply himp_star_frame; eauto.
+    eapply tuples0_Equiv; eauto.
   Qed.
 
   Theorem tree_leaf_fwd : forall len key sk ts (p : W), p = 0
@@ -126,21 +268,109 @@ Defined.
 
 Definition newS := SPEC("extra_stack", "len", "key") reserving 7
   PRE[V] [| V "len" >= $2 |] * [| V "key" < V "len" |] * mallocHeap 0
-  POST[R] tuples1 (V "len") Empty R * mallocHeap 0.
+  POST[R] tuples1 (V "len") (V "key") Empty R * mallocHeap 0.
 
-Definition m := bimport [[ "malloc"!"malloc" @ [mallocS], "malloc"!"free" @ [freeS] ]]
+Definition insertS := SPEC("extra_stack", "self", "tup") reserving 21
+  Al len, Al key, Al ts, Al t, Al ts',
+  PRE[V] tuples1 len key ts (V "self") * tuple t (V "tup") * [| length t = wordToNat len |] * mallocHeap 0
+         * [| insert ts t ts' |]
+  POST[R] [| R = $0 |] * tuples1 len key ts' (V "self") * mallocHeap 0.
+
+Definition grabInserted (ts ts' : tuples) : tuples :=
+  fun t => Ensembles.In _ ts' t /\ ~Ensembles.In _ ts t.
+
+Definition m := bimport [[ "malloc"!"malloc" @ [mallocS], "malloc"!"free" @ [freeS],
+                           "ArrayTuple"!"get" @ [ArrayTupleF.getS],
+                           "Tuples0"!"new" @ [Tuples0F.newS], "Tuples0"!"insert" @ [Tuples0F.insertS] ]]
   bmodule "Tuples1" {{
     bfunction "new"("extra_stack", "len", "key") [newS]
       "extra_stack" <-- Call "malloc"!"malloc"(0, 3)
       [PRE[V, R] R =?> 3 * [| R <> 0 |] * [| freeable R 3 |]
               * [| (V "len" >= $2)%word |] * [| (V "key" < V "len")%word |]
-       POST[R'] tuples1 (V "len") Empty R'];;
+       POST[R'] tuples1 (V "len") (V "key") Empty R'];;
 
       "extra_stack" *<- "len";;
       "extra_stack" + 4 *<- "key";;
       "extra_stack" + 8 *<- 0;;
       Return "extra_stack"
     end
+
+    (*with bfunction "insert"("extra_stack", "self", "tup", "len", "key", "p", "k1", "k2") [insertS]
+      "len" <-* "self";;
+      "key" <-* "self" + 4;;
+      "self" <- "self" + 8;;
+      "p" <-* "self";;
+      "k1" <-- Call "ArrayTuple"!"get"("extra_stack", "tup", "key")
+      [Al ts, Al t, Al ts', Al sk,
+       PRE[V, R] V "self" =*> V "p" * tree (V "len") (V "key") sk ts (V "p") * tuple t (V "tup")
+         * [| length t = wordToNat (V "len") |] * [| (V "key" < V "len")%word |] * mallocHeap 0
+         * [| R = Array.sel t (V "key") |] * [| ($2 <= V "len")%word |] * [| insert ts t ts' |]
+       POST[R'] [| R' = $0 |] * Ex p, Ex sk',
+         V "self" =*> p * tree (V "len") (V "key") sk' ts' p * mallocHeap 0];;
+
+      [Al ts, Al t, Al ts', Al sk,
+       PRE[V] V "self" =*> V "p" * tree (V "len") (V "key") sk ts (V "p") * tuple t (V "tup")
+         * [| length t = wordToNat (V "len") |] * [| (V "key" < V "len")%word |] * mallocHeap 0
+         * [| V "k1" = Array.sel t (V "key") |] * [| ($2 <= V "len")%word |] * [| insert ts t ts' |]
+       POST[R] [| R = $0 |] * Ex p, Ex sk',
+         V "self" =*> p * tree (V "len") (V "key") sk' ts' p * mallocHeap 0]
+      While ("p" <> 0) {
+        "k2" <-* "p" + 4;;
+
+        If ("k1" = "k2") {
+          (* Found existing node for this key.  Add to its collection. *)
+          "k2" <-* "p" + 8;;
+          Call "Tuples0"!"insert"("extra_stack", "k2", "tup")
+          [PRE[_] Emp
+           POST[R] [| R = $0 |] ];;
+          Return 0
+        } else {
+          (* No match.  Proceed to appropriate subtree. *)
+          If ("k1" < "k2") {
+            "self" <- "p"
+          } else {
+            "self" <- "p" + 12
+          };;
+          "p" <-* "self"
+        }
+      };;
+
+      (* This key hasn't been added yet.  Create a new tree node for it. *)
+      "k2" <-- Call "Tuples0"!"new"("extra_stack", "len")
+      [Al ts, Al t, Al ts',
+       PRE[V, R] tuples0 (V "len") Empty R * [| empty ts |]
+         * V "self" =*> V "p" * tuple t (V "tup")
+         * [| length t = wordToNat (V "len") |] * [| (V "key" < V "len")%word |] * mallocHeap 0
+         * [| V "k1" = Array.sel t (V "key") |] * [| ($2 <= V "len")%word |] * [| insert ts t ts' |]
+       POST[R'] [| R' = $0 |] * Ex p, Ex sk',
+         V "self" =*> p * tree (V "len") (V "key") sk' ts' p * mallocHeap 0];;
+
+      Call "Tuples0"!"insert"("extra_stack", "k2", "tup")
+      [Al ts, Al t, Al ts',
+       PRE[V] tuples0 (V "len") ts' (V "k2") * [| empty ts |]
+         * V "self" =*> V "p"
+         * [| length t = wordToNat (V "len") |] * [| (V "key" < V "len")%word |] * mallocHeap 0
+         * [| V "k1" = Array.sel t (V "key") |] * [| ($2 <= V "len")%word |] * [| insert ts t ts' |]
+       POST[R] [| R = $0 |] * Ex p, Ex sk',
+         V "self" =*> p * tree (V "len") (V "key") sk' ts' p * mallocHeap 0];;
+
+      "p" <-- Call "malloc"!"malloc"(0, 4)
+      [Al ts, Al t, Al ts',
+       PRE[V, R] R =?> 4 * [| R <> 0 |] * [| empty ts |]
+         * tuples0 (V "len") ts' (V "k2")
+         * V "self" =*> V "p"
+         * [| length t = wordToNat (V "len") |] * [| (V "key" < V "len")%word |] * mallocHeap 0
+         * [| V "k1" = Array.sel t (V "key") |] * [| ($2 <= V "len")%word |] * [| insert ts t ts' |]
+       POST[R] [| R = $0 |] * Ex p, Ex sk',
+         V "self" =*> p * tree (V "len") (V "key") sk' ts' p * mallocHeap 0];;
+
+      "p" *<- 0;;
+      "p" + 4 *<- "k1";;
+      "p" + 8 *<- "k2";;
+      "p" + 12 *<- 0;;
+      "self" *<- "p";;
+      Return 0
+    end*)
   }}.
 
 Local Hint Extern 1 (@eq W _ _) => words.
@@ -152,12 +382,267 @@ Qed.
 
 Hint Resolve empty_Empty.
 
+Lemma bounded_keepLt : forall ts key k,
+  bounded ts
+  -> bounded (keepLt ts key k).
+Proof.
+  Equiv.
+Qed.
+
+Hint Immediate bounded_keepLt.
+
+Lemma insert_keepLt : forall ts t ts' key k1 k,
+  insert ts t ts'
+  -> k1 = Array.sel t key
+  -> k1 < k
+  -> insert (keepLt ts key k) t (keepLt ts' key k).
+Proof.
+  Equiv.
+  subst; simpl.
+  exists x; intuition (subst; simpl in *; auto).
+  apply H2 in H3; intuition (subst; simpl in * ).
+  apply H2; tauto.
+  firstorder.
+Qed.
+
+Hint Immediate insert_keepLt.
+
+Lemma Equiv_keepEq_lt : forall k1 k ts key ts' t,
+  insert ts t ts'
+  -> k1 <> k
+  -> k1 = Array.sel t key
+  -> Equiv (keepEq ts key k) (keepEq ts' key k).
+Proof.
+  Equiv.
+  subst.
+  apply H2 in H3; intuition (subst; simpl in * ).
+  tauto.
+Qed.
+
+Hint Immediate Equiv_keepEq_lt.
+
+Lemma Equiv_keepGt_lt : forall k1 k ts key ts' t,
+  insert ts t ts'
+  -> k1 < k
+  -> k1 = Array.sel t key
+  -> Equiv (keepGt ts key k) (keepGt ts' key k).
+Proof.
+  Equiv.
+  subst.
+  apply H2 in H3; intuition (subst; simpl in * ).
+  nomega.
+Qed.
+
+Hint Immediate Equiv_keepGt_lt.
+
+Lemma Equiv_keepEq_gt : forall k1 k ts key ts' t,
+  insert ts t ts'
+  -> k1 <> k
+  -> k1 = Array.sel t key
+  -> Equiv (keepEq ts key k) (keepEq ts' key k).
+Proof.
+  Equiv.
+  subst.
+  apply H2 in H3; intuition (subst; simpl in * ).
+  tauto.
+Qed.
+
+Hint Immediate Equiv_keepEq_lt.
+
+Lemma Equiv_keepLt_gt : forall k1 k ts key ts' t,
+  insert ts t ts'
+  -> k <= k1
+  -> k1 <> k
+  -> k1 = Array.sel t key
+  -> Equiv (keepLt ts key k) (keepLt ts' key k).
+Proof.
+  Equiv.
+  subst.
+  apply H3 in H4; intuition (subst; simpl in * ).
+  tauto.
+Qed.
+
+Hint Immediate Equiv_keepLt_gt.
+
+Lemma insert_keepGt : forall ts t ts' key k1 k,
+  insert ts t ts'
+  -> k1 = Array.sel t key
+  -> k <= k1
+  -> k1 <> k
+  -> insert (keepGt ts key k) t (keepGt ts' key k).
+Proof.
+  Equiv.
+  subst; simpl.
+  exists x; intuition (subst; simpl in *; auto).
+  apply H3 in H4; intuition (subst; simpl in * ).
+  apply H3; tauto.
+  destruct (weq (Array.sel t key) k); intuition.
+  firstorder.
+Qed.
+
+Hint Immediate insert_keepGt.
+
+Lemma insert_keepEq : forall ts t ts' key k1,
+  insert ts t ts'
+  -> k1 = Array.sel t key
+  -> insert (keepEq ts key k1) t (keepEq ts' key k1).
+Proof.
+  Equiv.
+  subst; simpl.
+  exists x; intuition (subst; simpl in *; auto).
+  apply H1 in H2; intuition (subst; simpl in * ).
+  apply H1; tauto.
+  firstorder.
+Qed.
+
+Hint Immediate insert_keepEq.
+
+Lemma Equiv_keepLt_eq : forall k ts key ts' t,
+  insert ts t ts'
+  -> k = Array.sel t key
+  -> Equiv (keepLt ts key k) (keepLt ts' key k).
+Proof.
+  Equiv.
+  subst.
+  apply H1 in H2; intuition (subst; simpl in * ).
+  nomega.
+Qed.
+
+Lemma Equiv_keepGt_eq : forall k ts key ts' t,
+  insert ts t ts'
+  -> k = Array.sel t key
+  -> Equiv (keepGt ts key k) (keepGt ts' key k).
+Proof.
+  Equiv.
+  subst.
+  apply H1 in H2; intuition (subst; simpl in * ).
+  nomega.
+Qed.
+
+Hint Immediate Equiv_keepLt_eq Equiv_keepGt_eq.
+
+Lemma insert_empty_Empty : forall ts t ts',
+  empty ts
+  -> insert ts t ts'
+  -> insert Empty t ts'.
+Proof.
+  Equiv.
+Qed.
+
+Hint Immediate insert_empty_Empty.
+
+Theorem keepEq_eq : forall ts t ts' key k,
+  insert ts t ts'
+  -> empty ts
+  -> k = Array.sel t key
+  -> Equiv ts' (keepEq ts' key k).
+Proof.
+  Equiv.
+  apply H2 in H3; intuition (subst; simpl in * ).
+  tauto.
+  firstorder.
+Qed.
+
+Hint Immediate keepEq_eq.
+
+Theorem empty_keepLt : forall ts t ts' key k1,
+  insert ts t ts'
+  -> empty ts
+  -> k1 = Array.sel t key
+  -> empty (keepLt ts' key k1).
+Proof.
+  Equiv.
+  intuition.
+  apply H2 in H4; intuition (subst; simpl in * ).
+  nomega.
+  eauto.
+Qed.
+
+Theorem empty_keepGt : forall ts t ts' key k1,
+  insert ts t ts'
+  -> empty ts
+  -> k1 = Array.sel t key
+  -> empty (keepGt ts' key k1).
+Proof.
+  Equiv.
+  intuition.
+  apply H2 in H4; intuition (subst; simpl in * ).
+  nomega.
+  eauto.
+Qed.
+
+Hint Immediate empty_keepLt empty_keepGt.
+
 Theorem ok : moduleOk m.
 Proof.
   vcgen.
 
-  Ltac t := sep hints; eauto.
+  Ltac unifyLocals :=
+    match goal with
+    | [ _ : interp _ (![?P1] ?x) |- interp _ (![?P2] ?x) ] =>
+      match P1 with
+      | context[locals _ ?vs1 ?y _] =>
+        match P2 with
+        | context[locals _ ?vs2 y _] => unify vs1 vs2; descend
+        end
+      end
+    | [ |- interp _ (![?P1] ?x ---> ![?P2] ?x)%PropX ] =>
+      match P1 with
+      | context[locals ?y ?vs1 _ _] =>
+        match P2 with
+        | context[locals y ?vs2 _ _] => unify vs1 vs2; descend
+        end
+      end
+    end.
 
+  Ltac descend' := descend;
+                  try match goal with
+                      | [ H : insert _ ?b _ |- context[insert _ ?b' _] ] =>
+                        unify b b'
+                      end.
+
+  Ltac tree_cong :=
+    repeat apply himp_star_frame; try ((apply tuples0_Equiv || apply tree_Equiv); solve [ eauto ]);
+    descend'; step hints; eauto.
+
+  Ltac t := solve [ enterFunction
+              || (post; evaluate hints; descend; try unifyLocals; repeat (step hints; descend'); eauto;
+                  try tree_cong) ].
+
+
+  t.
+  t.
+  t.
+  t.
+  t.
+  t.
+  t.
+  t.
+
+
+  t.
+  t.
+  t.
+  t.
+  t.
+  t.
+  t.
+  t.
+  t.
+  t.
+  t.
+  t.
+  t.
+  t.
+  t.
+  t.
+  t.
+  t.
+  t.
+  t.
+  t.
+  t.
+  t.
   t.
   t.
   t.
